Use Dafny's improved :-

src/StandardLibrary/StandardLibrary.dfy
@@ -28,6 +28,11 @@ module {:extern "STL"} StandardLibrary {
     {
       Failure(this.error)
     }
+    function method PropagateFailureTest(): TestResult
+      requires Failure?
+    {
+      TestFailure(this.error)
+    }
     function method Extract(): T
       requires Success?
     {
@@ -45,30 +50,42 @@ module {:extern "STL"} StandardLibrary {
     }
   }
 
-  function method RequireEqual<T(==)>(expected: T, actual: T): (r: Result<()>)
-      ensures r.Success? ==> expected == actual
+  datatype TestResult = TestSuccess | TestFailure(error: string)
+  {
+    predicate method IsFailure() {
+      TestFailure?
+    }
+    function method PropagateFailure(): TestResult
+      requires TestFailure?
+    {
+      this
+    }
+  }
+
+  function method RequireEqual<T(==)>(expected: T, actual: T): (r: TestResult)
+      ensures r.TestSuccess? ==> expected == actual
   {
     // TODO: Report message similar to "Expected ___ but got ___"
     // Blocked on https://github.com/dafny-lang/dafny/issues/450
     RequireWithMessage(expected == actual, "Failed equality")
   }
   
-  function method Require(b: bool): (r: Result<()>)
-      ensures r.Success? ==> b
+  function method Require(b: bool): (r: TestResult)
+      ensures r.TestSuccess? ==> b
   {
     RequireWithMessage(b, "Failed requirement")
   }
 
-  function method RequireFailure<T>(x: Result<T>): (r: Result<()>)
-      ensures r.Success? ==> x.Failure?
+  function method RequireFailure<T>(x: Result<T>): (r: TestResult)
+      ensures r.TestSuccess? ==> x.Failure?
   {
     RequireWithMessage(x.Failure?, "Expected failure, but got success")
   }
 
-  function method RequireWithMessage(b: bool, message: string): (r: Result<()>)
-      ensures r.Success? ==> b
+  function method RequireWithMessage(b: bool, message: string): (r: TestResult)
+      ensures r.TestSuccess? ==> b
   {
-    if b then Success(()) else Failure(message)
+    if b then TestSuccess else TestFailure(message)
   }
 
   function method Join<T>(ss: seq<seq<T>>, joiner: seq<T>): (s: seq<T>)
