test/Crypto/Signature.dfy
@@ -7,25 +7,25 @@ module TestSignature {
   import opened UInt = StandardLibrary.UInt
   import Signature
 
-  method YCompression(s: Signature.ECDSAParams, fieldSize: nat) returns (r: Result<()>) {
+  method YCompression(s: Signature.ECDSAParams, fieldSize: nat) returns (r: TestResult) {
     var res := Signature.ECDSA.KeyGen(s);
     if res == None {
-      return Failure("KeyGen failed");
+      return TestFailure("KeyGen failed");
     }
     var (public, secret) := res.get;
     // This is the declared postcondition of the natively implemented KenGen method, plus a condition
     // about zero-padding:
-    var _ :- Require(0 < |secret|);
-    var _ :- Require(|public| == 1 + (fieldSize + 7) / 8);  // 1 byte for y; x zero-padded up to the field size
-    var _ :- Require(public[0] == 2 || public[0] == 3);  // public key uses y compression
-    return Success(());
+    :- Require(0 < |secret|);
+    :- Require(|public| == 1 + (fieldSize + 7) / 8);  // 1 byte for y; x zero-padded up to the field size
+    :- Require(public[0] == 2 || public[0] == 3);  // public key uses y compression
+    return TestSuccess;
   }
 
-  method {:test} YCompression384() returns (r: Result<()>) {
+  method {:test} YCompression384() returns (r: TestResult) {
     r := YCompression(Signature.ECDSA_P384, 384);
   }
 
-  method {:test} YCompression256() returns (r: Result<()>) {
+  method {:test} YCompression256() returns (r: TestResult) {
     r := YCompression(Signature.ECDSA_P256, 256);
   }
 }
