test/Keyring/KMSKeyring.dfy
@@ -10,33 +10,33 @@ module TestKMSKeyring {
   import opened UInt = StandardLibrary.UInt
   import KMSKeyringDef
   import KMSUtils
-  method {:test} TestRegionParseValidInput() returns (r: Result<()>) {
+  method {:test} TestRegionParseValidInput() returns (r: TestResult) {
     var cmk := "arn:aws:kms:us-west-1:658956600833:key/b3537ef1-d8dc-4780-9f5a-55776cbb2f7f";
-    var _ :- Require(KMSUtils.ValidFormatCMK(cmk));
+    :- Require(KMSUtils.ValidFormatCMK(cmk));
     var res :- KMSKeyringDef.RegionFromKMSKeyARN(cmk);
     r := RequireEqual("us-west-1", res);
   }
-  method {:test} TestRegionParseValidInputWildPartition() returns (r: Result<()>) {
+  method {:test} TestRegionParseValidInputWildPartition() returns (r: TestResult) {
     var cmk := "arn:xxx:kms:us-west-1:658956600833:key/b3537ef1-d8dc-4780-9f5a-55776cbb2f7f";
-    var _ :- Require(KMSUtils.ValidFormatCMK(cmk));
+    :- Require(KMSUtils.ValidFormatCMK(cmk));
     var res :- KMSKeyringDef.RegionFromKMSKeyARN(cmk);
     r := RequireEqual("us-west-1", res);
   }
-  method {:test} TestRegionParseValidInputNoPartition() returns (r: Result<()>) {
+  method {:test} TestRegionParseValidInputNoPartition() returns (r: TestResult) {
     var cmk := "arn::kms:us-west-1:658956600833:key/b3537ef1-d8dc-4780-9f5a-55776cbb2f7f";
-    var _ :- Require(KMSUtils.ValidFormatCMK(cmk));
+    :- Require(KMSUtils.ValidFormatCMK(cmk));
     var res :- KMSKeyringDef.RegionFromKMSKeyARN(cmk);
     r := RequireEqual("us-west-1", res);
   }
-  method {:test} TestRegionParseValidInputAliasArn() returns (r: Result<()>) {
+  method {:test} TestRegionParseValidInputAliasArn() returns (r: TestResult) {
     var cmk := "arn:aws:kms:us-west-1:658956600833:alias/EncryptDecrypt";
-    var _ :- Require(KMSUtils.ValidFormatCMK(cmk));
+    :- Require(KMSUtils.ValidFormatCMK(cmk));
     var res :- KMSKeyringDef.RegionFromKMSKeyARN(cmk);
     r := RequireEqual("us-west-1", res);
   }
-  method {:test} TestRegionParseBadInputAlias() returns (r: Result<()>) {
+  method {:test} TestRegionParseBadInputAlias() returns (r: TestResult) {
     var cmk := "alias/EncryptDecrypt";
-    var _ :- Require(KMSUtils.ValidFormatCMK(cmk));
+    :- Require(KMSUtils.ValidFormatCMK(cmk));
     var res := KMSKeyringDef.RegionFromKMSKeyARN(cmk);
     r := Require(res.Failure? && res.error == "Malformed ARN");
   }
