test/SDK/Keyring/RawAESKeyring.dfy
@@ -21,7 +21,7 @@ module TestAESKeyring {
   import UTF8
   import TestUtils
 
-  method {:test} TestOnEncryptOnDecryptGenerateDataKey() returns (r: Result<()>)
+  method {:test} TestOnEncryptOnDecryptGenerateDataKey() returns (r: TestResult)
   {
     var name :- UTF8.Encode("test Name");
     var namespace :- UTF8.Encode("test Namespace");
@@ -30,12 +30,12 @@ module TestAESKeyring {
     var valA :- UTF8.Encode("valA");
     var encryptionContext := [(keyA, valA)];
     var isValidAAD := MessageHeader.ComputeValidAAD(encryptionContext);
-    var _ :- Require(isValidAAD);
+    :- Require(isValidAAD);
 
     var wrappingAlgorithmID := AlgorithmSuite.AES_256_GCM_IV12_TAG16_HKDF_SHA384_ECDSA_P384;
 
     var onEncryptResult :- rawAESKeyring.OnEncrypt(wrappingAlgorithmID, encryptionContext, None);
-    var _ :- Require(onEncryptResult.Some? && |onEncryptResult.get.encryptedDataKeys| == 1);
+    :- Require(onEncryptResult.Some? && |onEncryptResult.get.encryptedDataKeys| == 1);
 
     var pdk := onEncryptResult.get.plaintextDataKey;
     var edk := onEncryptResult.get.encryptedDataKeys[0];
@@ -44,7 +44,7 @@ module TestAESKeyring {
     r := Require(res.Some? && res.get.plaintextDataKey == pdk);
   }
 
-  method {:test} TestOnEncryptOnDecryptSuppliedDataKey() returns (r: Result<()>)
+  method {:test} TestOnEncryptOnDecryptSuppliedDataKey() returns (r: TestResult)
   {
     var name :- UTF8.Encode("test Name");
     var namespace :- UTF8.Encode("test Namespace");
@@ -53,14 +53,14 @@ module TestAESKeyring {
     var valA :- UTF8.Encode("valA");
     var encryptionContext := [(keyA, valA)];
     var isValidAAD := MessageHeader.ComputeValidAAD(encryptionContext);
-    var _ :- Require(isValidAAD);
+    :- Require(isValidAAD);
 
     var pdk := seq(32, i => 0);
 
     var wrappingAlgorithmID := AlgorithmSuite.AES_256_GCM_IV12_TAG16_HKDF_SHA384_ECDSA_P384;
 
     var onEncryptResult :- rawAESKeyring.OnEncrypt(wrappingAlgorithmID, encryptionContext, Some(pdk));
-    var _ :- Require(onEncryptResult.Some? && |onEncryptResult.get.encryptedDataKeys| == 1);
+    :- Require(onEncryptResult.Some? && |onEncryptResult.get.encryptedDataKeys| == 1);
 
     var edk := onEncryptResult.get.encryptedDataKeys[0];
 
@@ -68,7 +68,7 @@ module TestAESKeyring {
     r := Require(res.Some? && res.get.plaintextDataKey == pdk);
   }
 
-  method {:test} TestOnDecryptNoEDKs() returns (r: Result<()>)
+  method {:test} TestOnDecryptNoEDKs() returns (r: TestResult)
   {
     var name :- UTF8.Encode("test Name");
     var namespace :- UTF8.Encode("test Namespace");
@@ -82,7 +82,7 @@ module TestAESKeyring {
     r := Require(res.None?);
   }
 
-  method {:test} TestOnEncryptUnserializableEC() returns (r: Result<()>)
+  method {:test} TestOnEncryptUnserializableEC() returns (r: TestResult)
   {
     var name :- UTF8.Encode("test Name");
     var namespace :- UTF8.Encode("test Namespace");
@@ -90,14 +90,14 @@ module TestAESKeyring {
     var keyA :- UTF8.Encode("keyA");
     var unserializableEncryptionContext := generateUnserializableEncryptionContext(keyA);
     var isValidAAD := MessageHeader.ComputeValidAAD(unserializableEncryptionContext);
-    var _ :- Require(!isValidAAD);
+    :- Require(!isValidAAD);
 
     var wrappingAlgorithmID := AlgorithmSuite.AES_256_GCM_IV12_TAG16_HKDF_SHA384_ECDSA_P384;
     var onEncryptResult := rawAESKeyring.OnEncrypt(wrappingAlgorithmID, unserializableEncryptionContext, None);
     r := Require(onEncryptResult.Failure?);
   }
 
-  method {:test} TestOnDecryptUnserializableEC() returns (r: Result<()>)
+  method {:test} TestOnDecryptUnserializableEC() returns (r: TestResult)
   {
     // Set up valid EDK for decryption
     var name :- UTF8.Encode("test Name");
@@ -108,30 +108,30 @@ module TestAESKeyring {
     var encryptionContext := [(keyA, valA)];
     var wrappingAlgorithmID := AlgorithmSuite.AES_256_GCM_IV12_TAG16_HKDF_SHA384_ECDSA_P384;
     var onEncryptResult :- rawAESKeyring.OnEncrypt(wrappingAlgorithmID, encryptionContext, None);
-    var _ :- Require(onEncryptResult.Some?);
-    var _ :- Require(|onEncryptResult.get.encryptedDataKeys| == 1);
+    :- Require(onEncryptResult.Some?);
+    :- Require(|onEncryptResult.get.encryptedDataKeys| == 1);
     var edk := onEncryptResult.get.encryptedDataKeys[0];
 
     // Set up EC that can't be serialized
     var unserializableEncryptionContext := generateUnserializableEncryptionContext(keyA);
     var isValidAAD := MessageHeader.ComputeValidAAD(unserializableEncryptionContext);
-    var _ :- Require(!isValidAAD);
+    :- Require(!isValidAAD);
 
     var onDecryptResult := rawAESKeyring.OnDecrypt(wrappingAlgorithmID, unserializableEncryptionContext, [edk]);
     r := Require(onDecryptResult.Failure?);
   }
 
-  method {:test} TestDeserializeEDKCiphertext() returns (r: Result<()>) {
+  method {:test} TestDeserializeEDKCiphertext() returns (r: TestResult) {
     var ciphertext := [0, 1, 2, 3];
     var authTag := [4, 5, 6, 7];
     var serializedEDKCiphertext := ciphertext + authTag;
     var encOutput := RawAESKeyringDef.DeserializeEDKCiphertext(serializedEDKCiphertext, |authTag|);
 
-    var _ :- RequireEqual(encOutput.cipherText, ciphertext);
+    :- RequireEqual(encOutput.cipherText, ciphertext);
     r := RequireEqual(encOutput.authTag, authTag);
   }
 
-  method {:test} TestSerializeEDKCiphertext() returns (r: Result<()>) {
+  method {:test} TestSerializeEDKCiphertext() returns (r: TestResult) {
     var ciphertext := [0, 1, 2, 3];
     var authTag := [4, 5, 6, 7];
     var encOutput := AESEncryption.EncryptionOutput(ciphertext, authTag);
