test/SDK/MessageHeader.dfy
@@ -14,13 +14,13 @@ module TestMessageHeader {
   import MessageHeader
   import TestUtils
   
-  method {:test} TestComputeValidAADEmpty() returns (r: Result<()>) {
+  method {:test} TestComputeValidAADEmpty() returns (r: TestResult) {
     var kvPairs := [];
     var valid := MessageHeader.ComputeValidAAD(kvPairs);
     r := Require(valid);
   }
 
-  method {:test} TestComputeValidAADOnePair() returns (r: Result<()>) {
+  method {:test} TestComputeValidAADOnePair() returns (r: TestResult) {
     var keyA :- UTF8.Encode("keyA");
     var valA :- UTF8.Encode("valA");
     var kvPairs := [(keyA, valA)];
@@ -28,7 +28,7 @@ module TestMessageHeader {
     r := Require(valid);
   }
 
-  method {:test} TestComputeValidAADOnePairMaxSize() returns (r: Result<()>) {
+  method {:test} TestComputeValidAADOnePairMaxSize() returns (r: TestResult) {
     var keyA :- UTF8.Encode("A");
     // (2^16 - 1) - 2 => 65533 what we want the size of the key value pair to fill
     // 65533 - 2 - 1 - 2 => 65528 is the size that we want the value to fill
@@ -39,7 +39,7 @@ module TestMessageHeader {
     r := Require(valid);
   }
 
-  method {:test} TestComputeValidAADMaxPairs() returns (r: Result<()>) {
+  method {:test} TestComputeValidAADMaxPairs() returns (r: TestResult) {
     var keyA :- UTF8.Encode("A");
     var valA :- UTF8.Encode("A");
     // (2^16 - 1) / (minimum kvPair size) => (2^16 - 1) / 6 => 10922 is the max
@@ -49,7 +49,7 @@ module TestMessageHeader {
     r := Require(valid);
   }
 
-  method {:test} TestComputeValidAADTooManyEntries() returns (r: Result<()>) {
+  method {:test} TestComputeValidAADTooManyEntries() returns (r: TestResult) {
     var keyA :- UTF8.Encode("keyA");
     var valA :- UTF8.Encode("valA");
     var kvPairs := seq(0x1_0000, _ => (keyA, valA));
@@ -57,7 +57,7 @@ module TestMessageHeader {
     r := Require(!valid);
   }
 
-  method {:test} TestComputeValidAADTooLarge() returns (r: Result<()>) {
+  method {:test} TestComputeValidAADTooLarge() returns (r: TestResult) {
     var keyA :- UTF8.Encode("keyA");
     var valA :- UTF8.Encode("valA");
     var kvPairs := seq(0x1_FFFF, _ => (keyA, valA));
@@ -65,7 +65,7 @@ module TestMessageHeader {
     r := Require(!valid);
   }
 
-  method {:test} TestComputeValidAADPairTooBig() returns (r: Result<()>) {
+  method {:test} TestComputeValidAADPairTooBig() returns (r: TestResult) {
     var keyA :- UTF8.Encode("keyA");
     var invalidVal := seq(0x1_0000, _ => 0);
     var kvPairs :=[(keyA, invalidVal)];
@@ -74,7 +74,7 @@ module TestMessageHeader {
     r := Require(!valid);
   }
 
-  method {:test} TestComputeValidAADUnsorted() returns (r: Result<()>) {
+  method {:test} TestComputeValidAADUnsorted() returns (r: TestResult) {
     var keyA :- UTF8.Encode("keyA");
     var valA :- UTF8.Encode("valA");
     var keyB :- UTF8.Encode("keyB");
@@ -84,14 +84,14 @@ module TestMessageHeader {
     r := Require(!valid);
   }
 
-  method {:test} TestComputeKVPairsLengthEmpty() returns (r: Result<()>) {
+  method {:test} TestComputeKVPairsLengthEmpty() returns (r: TestResult) {
     var kvPairs := [];
 
     var len := MessageHeader.ComputeKVPairsLength(kvPairs);
     r := RequireEqual(len as int, 0);
   }
 
-  method {:test} TestComputeKVPairsLengthOnePair() returns (r: Result<()>) {
+  method {:test} TestComputeKVPairsLengthOnePair() returns (r: TestResult) {
     var keyA :- UTF8.Encode("keyA");
     var valA :- UTF8.Encode("valA");
     var kvPairs := [(keyA, valA)];
@@ -101,7 +101,7 @@ module TestMessageHeader {
     r := RequireEqual(len as int, |expectedSerialization|);
   }
 
-  method {:test} TestComputeKVPairsLengthLong() returns (r: Result<()>) {
+  method {:test} TestComputeKVPairsLengthLong() returns (r: TestResult) {
     var keyA :- UTF8.Encode("A");
     var largeVal := seq(0x1_0000, _ => 0);
     TestUtils.AssumeLongSeqIsValidUTF8(largeVal);
