test/StandardLibrary/Base64.dfy
@@ -23,253 +23,253 @@ module TestBase64 {
     ensures forall i :: 0 <= i < |BASE64_TEST_VECTORS_ENCODED| ==> IsBase64String(BASE64_TEST_VECTORS_ENCODED[i])
   {}
 
-  method {:test} TestIsBase64CharSuccess() returns (r: Result<()>) {
+  method {:test} TestIsBase64CharSuccess() returns (r: TestResult) {
     r := Require(forall c :: c in BASE64_CHARS ==> IsBase64Char(c));
   }
 
-  method {:test} TestIsBase64CharFailure() returns (r: Result<()>) {
+  method {:test} TestIsBase64CharFailure() returns (r: TestResult) {
     r := Require(forall c :: c !in BASE64_CHARS ==> !IsBase64Char(c));
   }
 
-  method {:test} TestIsUnpaddedBase64StringSuccess() returns (r: Result<()>) {
+  method {:test} TestIsUnpaddedBase64StringSuccess() returns (r: TestResult) {
     r := Require(IsUnpaddedBase64String("VGVz"));
   }
 
-  method {:test} TestIsUnpaddedBase64StringTooShort() returns (r: Result<()>) {
+  method {:test} TestIsUnpaddedBase64StringTooShort() returns (r: TestResult) {
     r := Require(!IsUnpaddedBase64String("VGV"));
   }
 
-  method {:test} TestIsUnpaddedBase64StringNotBase64() returns (r: Result<()>) {
+  method {:test} TestIsUnpaddedBase64StringNotBase64() returns (r: TestResult) {
     r := Require(!IsUnpaddedBase64String("VGV$"));
   }
 
-  method {:test} TestIndexToChar63() returns (r: Result<()>) {
+  method {:test} TestIndexToChar63() returns (r: TestResult) {
     r := RequireEqual(IndexToChar(63), '/');
   }
 
-  method {:test} TestIndexToChar62() returns (r: Result<()>) {
+  method {:test} TestIndexToChar62() returns (r: TestResult) {
     r := RequireEqual(IndexToChar(62), '+');
   }
 
-  method {:test} TestIndexToCharDigits() returns (r: Result<()>) {
+  method {:test} TestIndexToCharDigits() returns (r: TestResult) {
     var digits := "0123456789";
     r := Require(forall i :: 52 <= i <= 61 ==> IndexToChar(i) in digits);
   }
 
-  method {:test} TestIndexToCharLowercase() returns (r: Result<()>) {
+  method {:test} TestIndexToCharLowercase() returns (r: TestResult) {
     var lowercase := "abcdefghijklmnopqrstuvwxyz";
     r := Require(forall i :: 26 <= i <= 51 ==> IndexToChar(i) in lowercase);
   }
 
-  method {:test} TestIndexToCharUppercase() returns (r: Result<()>) {
+  method {:test} TestIndexToCharUppercase() returns (r: TestResult) {
     var uppercase := "ABCDEFGHIJKLMNOPQRSTUVWXYZ";
     r := Require(forall i :: 0 <= i <= 25 ==> IndexToChar(i) in uppercase);
   }
 
-  method {:test} TestCharToIndex63() returns (r: Result<()>) {
+  method {:test} TestCharToIndex63() returns (r: TestResult) {
     r := RequireEqual(CharToIndex('/'), 63);
   }
 
-  method {:test} TestCharToIndex62() returns (r: Result<()>) {
+  method {:test} TestCharToIndex62() returns (r: TestResult) {
     r := RequireEqual(CharToIndex('+'), 62);
   }
 
-  method {:test} TestCharToIndexDigits() returns (r: Result<()>) {
+  method {:test} TestCharToIndexDigits() returns (r: TestResult) {
     var digits := "0123456789";
     r := Require(forall i :: 0 <= i < |digits| ==> CharToIndex(digits[i]) == ((i + 52) as index));
   }
 
-  method {:test} TestCharToIndexLowercase() returns (r: Result<()>) {
+  method {:test} TestCharToIndexLowercase() returns (r: TestResult) {
     var lowercase := "abcdefghijklmnopqrstuvwxyz";
     r := Require(forall i :: 0 <= i < |lowercase| ==> CharToIndex(lowercase[i]) == ((i + 26) as index));
   }
 
-  method {:test} TestCharToIndexUppercase() returns (r: Result<()>) {
+  method {:test} TestCharToIndexUppercase() returns (r: TestResult) {
     var uppercase := "ABCDEFGHIJKLMNOPQRSTUVWXYZ";
     r := Require(forall i :: 0 <= i < |uppercase| ==> CharToIndex(uppercase[i]) == (i as index));
   }
 
-  method {:test} TestUInt24ToSeq() returns (r: Result<()>) {
+  method {:test} TestUInt24ToSeq() returns (r: TestResult) {
     var input: uint24 := 0x100101;
     var output := [0x10, 0x01, 0x01];
     r := RequireEqual(output, UInt24ToSeq(input));
   }
 
-  method {:test} TestSeqToUInt24() returns (r: Result<()>) {
+  method {:test} TestSeqToUInt24() returns (r: TestResult) {
     var input := [0x10, 0x01, 0x01];
     var output: uint24 := 0x100101;
     r := RequireEqual(output, SeqToUInt24(input));
   }
 
-  method {:test} TestUInt24ToIndexSeq() returns (r: Result<()>) {
+  method {:test} TestUInt24ToIndexSeq() returns (r: TestResult) {
     var input: uint24 := 0x100101;
     var output := [0x04, 0x00, 0x04, 0x01];
     r := RequireEqual(output, UInt24ToIndexSeq(input));
   }
 
-  method {:test} TestIndexSeqToUInt24() returns (r: Result<()>) {
+  method {:test} TestIndexSeqToUInt24() returns (r: TestResult) {
     var input := [0x04, 0x00, 0x04, 0x01];
     var output: uint24 := 0x100101;
     r := RequireEqual(output, IndexSeqToUInt24(input));
   }
 
-  method {:test} TestDecodeBlock() returns (r: Result<()>) {
+  method {:test} TestDecodeBlock() returns (r: TestResult) {
     var input := [0x04, 0x00, 0x04, 0x01];
     var output := [0x10, 0x01, 0x01];
     r := RequireEqual(output, DecodeBlock(input));
   }
 
-  method {:test} TestEncodeBlock() returns (r: Result<()>) {
+  method {:test} TestEncodeBlock() returns (r: TestResult) {
     var input := [0x10, 0x01, 0x01];
     var output := [0x04, 0x00, 0x04, 0x01];
     r := RequireEqual(output, EncodeBlock(input));
   }
 
-  method {:test} TestDecodeRecursively() returns (r: Result<()>) {
+  method {:test} TestDecodeRecursively() returns (r: TestResult) {
     var input := [0x04, 0x00, 0x04, 0x01, 0x04, 0x00, 0x04, 0x01];
     var output := [0x10, 0x01, 0x01, 0x10, 0x01, 0x01];
     r := RequireEqual(output, DecodeRecursively(input));
   }
 
-  method {:test} TestEncodeRecursively() returns (r: Result<()>) {
+  method {:test} TestEncodeRecursively() returns (r: TestResult) {
     var input := [0x10, 0x01, 0x01, 0x10, 0x01, 0x01];
     var output := [0x04, 0x00, 0x04, 0x01, 0x04, 0x00, 0x04, 0x01];
     r := RequireEqual(output, EncodeRecursively(input));
   }
 
-  method {:test} TestFromCharsToIndices() returns (r: Result<()>) {
+  method {:test} TestFromCharsToIndices() returns (r: TestResult) {
     var input := "aA1+/";
     var output := [0x1A, 0x00, 0x35, 0x3E, 0x3F];
     r := RequireEqual(output, FromCharsToIndices(input));
   }
 
-  method {:test} TestFromIndicesToChars() returns (r: Result<()>) {
+  method {:test} TestFromIndicesToChars() returns (r: TestResult) {
     var input := [0x1A, 0x00, 0x35, 0x3E, 0x3F];
     var output := "aA1+/";
     r := RequireEqual(output, FromIndicesToChars(input));
   }
 
-  method {:test} TestDecodeUnpadded() returns (r: Result<()>) {
+  method {:test} TestDecodeUnpadded() returns (r: TestResult) {
     var input := "VGVzdGluZysx";
     var output := [0x54, 0x65, 0x73, 0x74, 0x69, 0x6E, 0x67, 0x2B, 0x31];
     r := RequireEqual(output, DecodeUnpadded(input));
   }
 
-  method {:test} TestEncodeUnpadded() returns (r: Result<()>) {
+  method {:test} TestEncodeUnpadded() returns (r: TestResult) {
     var input := [0x54, 0x65, 0x73, 0x74, 0x69, 0x6E, 0x67, 0x2B, 0x31];
     var output := "VGVzdGluZysx";
     r := RequireEqual(output, EncodeUnpadded(input));
   }
 
-  method {:test} TestDecodeUnpaddedEmpty() returns (r: Result<()>) {
+  method {:test} TestDecodeUnpaddedEmpty() returns (r: TestResult) {
     r := RequireEqual([], DecodeUnpadded([]));
   }
 
-  method {:test} TestEncodeUnpaddedEmpty() returns (r: Result<()>) {
+  method {:test} TestEncodeUnpaddedEmpty() returns (r: TestResult) {
     r := RequireEqual([], EncodeUnpadded([]));
   }
 
-  method {:test} TestIs1PaddingSuccess() returns (r: Result<()>) {
+  method {:test} TestIs1PaddingSuccess() returns (r: TestResult) {
     r := Require(Is1Padding("VGU="));
   }
 
-  method {:test} TestIs1PaddingTooShort() returns (r: Result<()>) {
+  method {:test} TestIs1PaddingTooShort() returns (r: TestResult) {
     r := Require(!Is1Padding("VG="));
   }
 
-  method {:test} TestIs1PaddingTooLong() returns (r: Result<()>) {
+  method {:test} TestIs1PaddingTooLong() returns (r: TestResult) {
     r := Require(!Is1Padding("VGUU="));
   }
 
-  method {:test} TestIs1PaddingInvalidChar0() returns (r: Result<()>) {
+  method {:test} TestIs1PaddingInvalidChar0() returns (r: TestResult) {
     r := Require(!Is1Padding("$GU="));
   }
 
-  method {:test} TestIs1PaddingInvalidChar1() returns (r: Result<()>) {
+  method {:test} TestIs1PaddingInvalidChar1() returns (r: TestResult) {
     r := Require(!Is1Padding("V$U="));
   }
 
-  method {:test} TestIs1PaddingInvalidChar2() returns (r: Result<()>) {
+  method {:test} TestIs1PaddingInvalidChar2() returns (r: TestResult) {
     r := Require(!Is1Padding("VG$="));
   }
 
-  method {:test} TestIs1PaddingInvalidChar3() returns (r: Result<()>) {
+  method {:test} TestIs1PaddingInvalidChar3() returns (r: TestResult) {
     r := Require(!Is1Padding("VGVz"));
   }
 
-  method {:test} TestIs1PaddingInvalidChar2Modulus() returns (r: Result<()>) {
+  method {:test} TestIs1PaddingInvalidChar2Modulus() returns (r: TestResult) {
     r := Require(!Is1Padding("VGV="));
   }
 
-  method {:test} TestDecode1Padding() returns (r: Result<()>) {
+  method {:test} TestDecode1Padding() returns (r: TestResult) {
     var input := "VGU=";
     var output := [0x54, 0x65];
     r := RequireEqual(output, Decode1Padding(input));
   }
 
-  method {:test} TestEncode1Padding() returns (r: Result<()>) {
+  method {:test} TestEncode1Padding() returns (r: TestResult) {
     var input := [0x54, 0x65];
     var output := "VGU=";
     r := RequireEqual(output, Encode1Padding(input));
   }
 
-  method {:test} TestIs2PaddingSuccess() returns (r: Result<()>) {
+  method {:test} TestIs2PaddingSuccess() returns (r: TestResult) {
     r := Require(Is2Padding("VA=="));
   }
 
-  method {:test} TestIs2PaddingTooShort() returns (r: Result<()>) {
+  method {:test} TestIs2PaddingTooShort() returns (r: TestResult) {
     r := Require(!Is2Padding("VA="));
   }
 
-  method {:test} TestIs2PaddingTooLong() returns (r: Result<()>) {
+  method {:test} TestIs2PaddingTooLong() returns (r: TestResult) {
     r := Require(!Is2Padding("VAA=="));
   }
 
-  method {:test} TestIs2PaddingInvalidChar0() returns (r: Result<()>) {
+  method {:test} TestIs2PaddingInvalidChar0() returns (r: TestResult) {
     r := Require(!Is2Padding("$A=="));
   }
 
-  method {:test} TestIs2PaddingInvalidChar1() returns (r: Result<()>) {
+  method {:test} TestIs2PaddingInvalidChar1() returns (r: TestResult) {
     r := Require(!Is2Padding("V$=="));
   }
 
-  method {:test} TestIs2PaddingInvalidChar2() returns (r: Result<()>) {
+  method {:test} TestIs2PaddingInvalidChar2() returns (r: TestResult) {
     r := Require(!Is2Padding("VAA="));
   }
 
-  method {:test} TestIs2PaddingInvalidChar3() returns (r: Result<()>) {
+  method {:test} TestIs2PaddingInvalidChar3() returns (r: TestResult) {
     r := Require(!Is2Padding("VA=A"));
   }
 
-  method {:test} TestIs2PaddingInvalidChar1Modulus() returns (r: Result<()>) {
+  method {:test} TestIs2PaddingInvalidChar1Modulus() returns (r: TestResult) {
     r := Require(!Is2Padding("VB=="));
   }
 
-  method {:test} TestDecode2Padding() returns (r: Result<()>) {
+  method {:test} TestDecode2Padding() returns (r: TestResult) {
     var input := "VA==";
     var output := [0x54];
     r := RequireEqual(output, Decode2Padding(input));
   }
 
-  method {:test} TestEncode2Padding() returns (r: Result<()>) {
+  method {:test} TestEncode2Padding() returns (r: TestResult) {
     var input := [0x54];
     var output := "VA==";
     r := RequireEqual(output, Encode2Padding(input));
   }
 
-  method {:test} TestIsBase64StringTestVectors() returns (r: Result<()>) {
+  method {:test} TestIsBase64StringTestVectors() returns (r: TestResult) {
     r := Require(forall i :: i in BASE64_TEST_VECTORS_ENCODED ==> IsBase64String(i) == true);
   }
 
-  method {:test} TestIsBase64StringBadLength() returns (r: Result<()>) {
+  method {:test} TestIsBase64StringBadLength() returns (r: TestResult) {
     r := Require(!IsBase64String("VG="));
   }
 
-  method {:test} TestIsBase64StringBadString() returns (r: Result<()>) {
+  method {:test} TestIsBase64StringBadString() returns (r: TestResult) {
     r := Require(!IsBase64String("VC=="));
   }
 
-  method {:test} TestSanityCheckDecodedTestVectors() returns (r: Result<()>) {
+  method {:test} TestSanityCheckDecodedTestVectors() returns (r: TestResult) {
 
     var testVectorIndex := 0;
     while testVectorIndex < |BASE64_TEST_VECTORS_DECODED|
@@ -284,37 +284,37 @@ module TestBase64 {
         uint8Message := uint8Message + [strMessage[msgIndex] as uint8];
         msgIndex := msgIndex + 1;
       }
-      var _ :- RequireEqual(BASE64_TEST_VECTORS_DECODED_UINT8[testVectorIndex], uint8Message);
+      :- RequireEqual(BASE64_TEST_VECTORS_DECODED_UINT8[testVectorIndex], uint8Message);
       testVectorIndex := testVectorIndex + 1;
     }
-    return Success(());
+    return TestSuccess;
   }
 
-  method {:test} TestDecodeValidTestVectors() returns (r: Result<()>) {
+  method {:test} TestDecodeValidTestVectors() returns (r: TestResult) {
     r := Require(forall i :: 0 <= i < |BASE64_TEST_VECTORS_ENCODED| ==>
       DecodeValid(BASE64_TEST_VECTORS_ENCODED[i]) == BASE64_TEST_VECTORS_DECODED_UINT8[i]);
   }
 
-  method {:test} TestDecodeTestVectors() returns (r: Result<()>) {
+  method {:test} TestDecodeTestVectors() returns (r: TestResult) {
     r := Require(forall i :: 0 <= i < |BASE64_TEST_VECTORS_ENCODED| ==>
       Decode(BASE64_TEST_VECTORS_ENCODED[i]) == Success(BASE64_TEST_VECTORS_DECODED_UINT8[i]));
   }
 
-  method {:test} TestDecodeFailure() returns (r: Result<()>) {
+  method {:test} TestDecodeFailure() returns (r: TestResult) {
     r := RequireEqual(Failure("The encoding is malformed"), Decode("$"));
   }
 
-  method {:test} TestEncode() returns (r: Result<()>) {
+  method {:test} TestEncode() returns (r: TestResult) {
     r := Require(forall i :: 0 <= i < |BASE64_TEST_VECTORS_DECODED_UINT8| ==>
       Encode(BASE64_TEST_VECTORS_DECODED_UINT8[i]) == BASE64_TEST_VECTORS_ENCODED[i]);
   }
 
-  method {:test} TestEncodeDecode() returns (r: Result<()>) {
+  method {:test} TestEncodeDecode() returns (r: TestResult) {
     r := Require(forall i :: 0 <= i < |BASE64_TEST_VECTORS_DECODED_UINT8| ==>
       Decode(Encode(BASE64_TEST_VECTORS_DECODED_UINT8[i])) == Success(BASE64_TEST_VECTORS_DECODED_UINT8[i]));
   }
 
-  method {:test} TestDecodeEncode() returns (r: Result<()>) {
+  method {:test} TestDecodeEncode() returns (r: TestResult) {
     r := Require(forall i :: 0 <= i < |BASE64_TEST_VECTORS_ENCODED| ==>
       (Decode(BASE64_TEST_VECTORS_ENCODED[i]).Success?
       && Encode(Decode(BASE64_TEST_VECTORS_ENCODED[i]).value) == BASE64_TEST_VECTORS_ENCODED[i]));
