test/StandardLibrary/StandardLibrary.dfy
@@ -3,115 +3,115 @@ include "../../src/StandardLibrary/StandardLibrary.dfy"
 module TestStandardLibrary {
   import opened StandardLibrary
 
-  method {:test} TestRequireFailure() returns (ret: Result<()>) {
+  method {:test} TestRequireFailure() returns (ret: TestResult) {
     var failure: Result<string> := Failure("Some failure");
-    var _ :- RequireFailure(failure);
+    :- RequireFailure(failure);
 
     var requireFailureGivenSuccess := RequireFailure(Success(()));
-    var _ :- Require(requireFailureGivenSuccess.Failure?);
-    ret := RequireFailure(requireFailureGivenSuccess);
+    :- Require(requireFailureGivenSuccess.TestFailure?);
+    ret := RequireFailure<()>(Failure(requireFailureGivenSuccess.error));
   }
 
-  method {:test} TestJoinMultiElementSeq() returns (ret: Result<()>) {
+  method {:test} TestJoinMultiElementSeq() returns (ret: TestResult) {
     var input := ["comma", "separated", "list"];
     var output := Join(input, ",");
     ret := RequireEqual("comma,separated,list", output);
   }
 
-  method {:test} TestJoinSingleElementSeq() returns (ret: Result<()>) {
+  method {:test} TestJoinSingleElementSeq() returns (ret: TestResult) {
     var input := ["one"];
     var output := Join(input, ",");
     ret := RequireEqual("one", output);
   }
 
-  method {:test} TestJoinSplit() returns (ret: Result<()>) {
+  method {:test} TestJoinSplit() returns (ret: TestResult) {
     var input := "comma,separated,list";
     var output := Join(Split(input, ','), ",");
     ret := RequireEqual(input, output);
   }
 
-  method {:test} TestSplitJoin() returns (ret: Result<()>) {
+  method {:test} TestSplitJoin() returns (ret: TestResult) {
     var input := ["comma", "separated", "list"];
     var output := Split(Join(input, ","), ',');
     ret := RequireEqual(input, output);
   }
 
-  method {:test} TestSplitByteSeq() returns (ret: Result<()>) {
+  method {:test} TestSplitByteSeq() returns (ret: TestResult) {
     var input := "comma,separated,list";
     var output := Split(input, ',');
     ret := RequireEqual(["comma", "separated", "list"], output);
   }
 
-  method {:test} TestSplitNumSeq() returns (ret: Result<()>) {
+  method {:test} TestSplitNumSeq() returns (ret: TestResult) {
     var input := [1, 2, 3, 0, 1, 2, 3];
     var output := Split(input, 0);
     ret := RequireEqual([[1, 2, 3], [1, 2, 3]], output);
   }
 
-  method {:test} TestSplitFinalElementDelim() returns (ret: Result<()>) {
+  method {:test} TestSplitFinalElementDelim() returns (ret: TestResult) {
     var input := "one,";
     var output := Split(input, ',');
     ret := RequireEqual(["one", ""], output);
   }
 
-  method {:test} TestSplitNoDelim() returns (ret: Result<()>) {
+  method {:test} TestSplitNoDelim() returns (ret: TestResult) {
     var input := "no comma";
     var output := Split(input, ',');
     ret := RequireEqual(["no comma"], output);
   }
 
-  method {:test} TestSplitOnlyElemIsDelim() returns (ret: Result<()>) {
+  method {:test} TestSplitOnlyElemIsDelim() returns (ret: TestResult) {
     var input := ",";
     var output := Split(input, ',');
     ret := RequireEqual(["", ""], output);
   }
 
-  method {:test} TestSplitEmpty() returns (ret: Result<()>) {
+  method {:test} TestSplitEmpty() returns (ret: TestResult) {
     var input := "";
     var output := Split(input, ',');
     ret := RequireEqual([""], output);
   }
 
-  method {:test} TestFindIndexMatchingSimple() returns (ret: Result<()>) {
+  method {:test} TestFindIndexMatchingSimple() returns (ret: TestResult) {
     var input := "abcd";
     var output := FindIndexMatching(input, 'c', 0);
     ret := RequireEqual(Some(2), output);
   }
 
-  method {:test} TestFindIndexMatchingDuplicates() returns (ret: Result<()>) {
+  method {:test} TestFindIndexMatchingDuplicates() returns (ret: TestResult) {
     var input := "abcdc";
     var output := FindIndexMatching(input, 'c', 0);
     ret := RequireEqual(Some(2), output);
   }
 
-  method {:test} TestFindIndexMatchingNone() returns (ret: Result<()>) {
+  method {:test} TestFindIndexMatchingNone() returns (ret: TestResult) {
     var input := "abcd";
     var output := FindIndexMatching(input, 'e', 0);
     ret := RequireEqual(None, output);
   }
 
-  method {:test} TestFindIndexSimple() returns (ret: Result<()>)
+  method {:test} TestFindIndexSimple() returns (ret: TestResult)
   {
     var input := "abcd";
     var output := FindIndex(input, x => x == 'c', 0);
     ret := RequireEqual(Some(2), output);
   }
 
-  method {:test} TestFindIndexComplex() returns (ret: Result<()>)
+  method {:test} TestFindIndexComplex() returns (ret: TestResult)
   {
     var input := "abcd";
     var output := FindIndex(input, x => x in "crepe", 0);
     ret := RequireEqual(Some(2), output);
   }
 
-  method {:test} TestFindIndexDuplicates() returns (ret: Result<()>)
+  method {:test} TestFindIndexDuplicates() returns (ret: TestResult)
   {
     var input := "abcdc";
     var output := FindIndex(input, x => x == 'c', 0);
     ret := RequireEqual(Some(2), output);
   }
 
-  method {:test} TestFindIndexNone() returns (ret: Result<()>)
+  method {:test} TestFindIndexNone() returns (ret: TestResult)
   {
     var input := "abcd";
     var output := FindIndex(input, x => false, 0);
@@ -122,41 +122,41 @@ module TestStandardLibrary {
     entry in ["a"]
   }
 
-  method {:test} TestFilterSomeValid() returns (ret: Result<()>) {
+  method {:test} TestFilterSomeValid() returns (ret: TestResult) {
     var input := ["a", "b", "a"];
     var output := Filter(input, TestFilterPredicate);
     ret := RequireEqual(["a", "a"], output);
   }
 
-  method {:test} TestFilterNoneValid() returns (ret: Result<()>) {
+  method {:test} TestFilterNoneValid() returns (ret: TestResult) {
     var input := ["c", "b", "c"];
     var output := Filter(input, TestFilterPredicate);
     ret := RequireEqual([], output);
   }
 
-  method {:test} TestFilterNothing() returns (ret: Result<()>) {
+  method {:test} TestFilterNothing() returns (ret: TestResult) {
     var input := [];
     var output := Filter(input, TestFilterPredicate);
     ret := RequireEqual([], output);
   }
 
-  method {:test} TestMinPositives() returns (ret: Result<()>) {
+  method {:test} TestMinPositives() returns (ret: TestResult) {
     ret := RequireEqual(1, Min(1, 2));
   }
 
-  method {:test} TestMinNegatives() returns (ret: Result<()>) {
+  method {:test} TestMinNegatives() returns (ret: TestResult) {
     ret := RequireEqual(-2, Min(-1, -2));
   }
 
-  method {:test} TestMinPositivesNegatives() returns (ret: Result<()>) {
+  method {:test} TestMinPositivesNegatives() returns (ret: TestResult) {
     ret := RequireEqual(-1, Min(-1, 1));
   }
 
-  method {:test} TestMinDuplicateNumber() returns (ret: Result<()>) {
+  method {:test} TestMinDuplicateNumber() returns (ret: TestResult) {
     ret := RequireEqual(0, Min(0, 0));
   }
 
-  method {:test} TestSeqToArray() returns (ret: Result<()>) {
+  method {:test} TestSeqToArray() returns (ret: TestResult) {
     var input: seq<int> := [1, 2, 3];
     var output := SeqToArray(input);
 
@@ -165,13 +165,13 @@ module TestStandardLibrary {
     expected[1] := 2;
     expected[2] := 3;
 
-    var _ :- RequireEqual(expected.Length, output.Length);
-    var _ :- RequireEqual(expected[0], output[0]);
-    var _ :- RequireEqual(expected[1], output[1]);
+    :- RequireEqual(expected.Length, output.Length);
+    :- RequireEqual(expected[0], output[0]);
+    :- RequireEqual(expected[1], output[1]);
     ret := RequireEqual(expected[2], output[2]);
   }
 
-  method {:test} TestSeqToArrayEmpty() returns (ret: Result<()>) {
+  method {:test} TestSeqToArrayEmpty() returns (ret: TestResult) {
     var input: seq<char> := [];
     var output := SeqToArray(input);
     ret := RequireEqual(0, output.Length);
@@ -179,31 +179,31 @@ module TestStandardLibrary {
 
   predicate method TestStandardLibraryLessPredicate(a: int, b: int) { a < b }
 
-  method {:test} TestLexicographicLessOrEqualTrue() returns (ret: Result<()>) {
+  method {:test} TestLexicographicLessOrEqualTrue() returns (ret: TestResult) {
     var a: seq<int> := [1, 2, 3];
     var b: seq<int> := [1, 2, 4];
     ret := RequireEqual(true, LexicographicLessOrEqual(a, b, TestStandardLibraryLessPredicate));
   }
 
-  method {:test} TestLexicographicLessOrEqualFalse() returns (ret: Result<()>) {
+  method {:test} TestLexicographicLessOrEqualFalse() returns (ret: TestResult) {
     var a: seq<int> := [1, 2, 3];
     var b: seq<int> := [1, 2, 4];
     ret := RequireEqual(false, LexicographicLessOrEqual(b, a, TestStandardLibraryLessPredicate));
   }
 
-  method {:test} TestLexicographicLessOrEqualAllEqual() returns (ret: Result<()>) {
+  method {:test} TestLexicographicLessOrEqualAllEqual() returns (ret: TestResult) {
     var a: seq<int> := [1, 2, 3];
     var b: seq<int> := [1, 2, 3];
     ret := RequireEqual(true, LexicographicLessOrEqual(a, b, TestStandardLibraryLessPredicate));
   }
 
-  method {:test} TestLexicographicLessOrEqualNoneEqual() returns (ret: Result<()>) {
+  method {:test} TestLexicographicLessOrEqualNoneEqual() returns (ret: TestResult) {
     var a: seq<int> := [1];
     var b: seq<int> := [2];
     ret := RequireEqual(true, LexicographicLessOrEqual(a, b, TestStandardLibraryLessPredicate));
   }
 
-  method {:test} TestLexicographicLessOrEqualEmpty() returns (ret: Result<()>) {
+  method {:test} TestLexicographicLessOrEqualEmpty() returns (ret: TestResult) {
     var a: seq<int> := [];
     var b: seq<int> := [];
     ret := RequireEqual(true, LexicographicLessOrEqual(a, b, TestStandardLibraryLessPredicate));
