test/StandardLibrary/UInt.dfy
@@ -5,32 +5,32 @@ module TestUInt {
   import opened StandardLibrary
   import opened UInt = StandardLibrary.UInt
 
-  method {:test} TestUInt16ToSeq() returns (r: Result<()>) {
+  method {:test} TestUInt16ToSeq() returns (r: TestResult) {
     var x: uint16 := 0x0122;
     r := RequireEqual([0x01, 0x22], UInt16ToSeq(x));
   }
 
-  method {:test} TestSeqToUInt16() returns (r: Result<()>) {
+  method {:test} TestSeqToUInt16() returns (r: TestResult) {
     var s := [0x01, 0x22];
     r := RequireEqual(0x0122 as uint16, SeqToUInt16(s));
   }
 
-  method {:test} TestUInt32ToSeq() returns (r: Result<()>) {
+  method {:test} TestUInt32ToSeq() returns (r: TestResult) {
     var x := 0x01023044;
     r := RequireEqual([0x01, 0x02, 0x30, 0x44], UInt32ToSeq(x));
   }
 
-  method {:test} TestSeqToUInt32() returns (r: Result<()>) {
+  method {:test} TestSeqToUInt32() returns (r: TestResult) {
     var s := [0x01, 0x02, 0x30, 0x44];
     r := RequireEqual(0x01023044 as uint32, SeqToUInt32(s));
   }
 
-  method {:test} TestUInt64ToSeq() returns (r: Result<()>) {
+  method {:test} TestUInt64ToSeq() returns (r: TestResult) {
     var x: uint64 := 0x0102304455667788;
     r := RequireEqual([0x01, 0x02, 0x30, 0x44, 0x55, 0x66, 0x77, 0x88], UInt64ToSeq(x));
   }
 
-  method {:test} TestSeqToUInt64() returns (r: Result<()>) {
+  method {:test} TestSeqToUInt64() returns (r: TestResult) {
     var s := [0x01, 0x02, 0x30, 0x44, 0x55, 0x66, 0x77, 0x88];
     r := RequireEqual(0x0102304455667788 as uint64, SeqToUInt64(s));
   }
