test/Util/UTF8.dfy
@@ -6,169 +6,169 @@ module TestUTF8 {
   import opened UInt = StandardLibrary.UInt
   import opened UTF8
 
-  method {:test} TestEncodeHappyCase() returns (r: Result<()>) {
+  method {:test} TestEncodeHappyCase() returns (r: TestResult) {
     var unicodeString := "abc\u0306\u01FD\u03B2";
     var expectedBytes := [0x61, 0x62, 0x63, 0xCC, 0x86, 0xC7, 0xBD, 0xCE, 0xB2];
     var encoded :- UTF8.Encode(unicodeString);
     r := RequireEqual(expectedBytes, encoded);
   }
 
-  method {:test} TestEncodeInvalidUnicode() returns (r: Result<()>) {
+  method {:test} TestEncodeInvalidUnicode() returns (r: TestResult) {
     // Create string with UTF-16 surrogate (\uD800)
     var invalidUnicode := "abc\uD800";
     var encoded := UTF8.Encode(invalidUnicode);
     r := RequireFailure(encoded);
   }
 
-  method {:test} TestDecodeHappyCase() returns (r: Result<()>) {
+  method {:test} TestDecodeHappyCase() returns (r: TestResult) {
     var unicodeBytes := [0x61, 0x62, 0x63, 0xCC, 0x86, 0xC7, 0xBD, 0xCE, 0xB2];
     var expectedString := "abc\u0306\u01FD\u03B2";
     var decoded :- UTF8.Decode(unicodeBytes);
     r := RequireEqual(expectedString, decoded);
   }
 
-  method {:test} TestDecodeInvalidUnicode() returns (r: Result<()>) {
+  method {:test} TestDecodeInvalidUnicode() returns (r: TestResult) {
     // Create byte sequence with UTF-16 surrogate (0xEDA080)
     var invalidUnicode := [0x61, 0x62, 0x63, 0xED, 0xA0, 0x80];
     r := Require(!ValidUTF8Seq(invalidUnicode));
   }
 
-  method {:test} Test1Byte() returns (r: Result<()>) {
+  method {:test} Test1Byte() returns (r: TestResult) {
     // Null
     var decoded := "\u0000";
     var encoded :- UTF8.Encode(decoded);
-    var _ :- RequireEqual([0x00], encoded);
-    var _ :- Require(Uses1Byte(encoded));
+    :- RequireEqual([0x00], encoded);
+    :- Require(Uses1Byte(encoded));
     var redecoded :- UTF8.Decode(encoded);
-    var _ :- RequireEqual(decoded, redecoded);
+    :- RequireEqual(decoded, redecoded);
 
     // Space
     decoded := "\u0020";
     encoded :- UTF8.Encode(decoded);
-    var _ :- RequireEqual([0x20], encoded);
-    var _ :- Require(Uses1Byte(encoded));
+    :- RequireEqual([0x20], encoded);
+    :- Require(Uses1Byte(encoded));
     redecoded :- UTF8.Decode(encoded);
-    var _ :- RequireEqual(decoded, redecoded);
+    :- RequireEqual(decoded, redecoded);
 
     decoded := "$";
     encoded :- UTF8.Encode(decoded);
-    var _ :- RequireEqual([0x24], encoded);
-    var _ :- Require(Uses1Byte(encoded));
+    :- RequireEqual([0x24], encoded);
+    :- Require(Uses1Byte(encoded));
     redecoded :- UTF8.Decode(encoded);
-    var _ :- RequireEqual(decoded, redecoded);
+    :- RequireEqual(decoded, redecoded);
 
     decoded := "0";
     encoded :- UTF8.Encode(decoded);
-    var _ :- RequireEqual([0x30], encoded);
-    var _ :- Require(Uses1Byte(encoded));
+    :- RequireEqual([0x30], encoded);
+    :- Require(Uses1Byte(encoded));
     redecoded :- UTF8.Decode(encoded);
-    var _ :- RequireEqual(decoded, redecoded);
+    :- RequireEqual(decoded, redecoded);
 
     decoded := "A";
     encoded :- UTF8.Encode(decoded);
-    var _ :- RequireEqual([0x41], encoded);
-    var _ :- Require(Uses1Byte(encoded));
+    :- RequireEqual([0x41], encoded);
+    :- Require(Uses1Byte(encoded));
     redecoded :- UTF8.Decode(encoded);
-    var _ :- RequireEqual(decoded, redecoded);
+    :- RequireEqual(decoded, redecoded);
 
     decoded := "a";
     encoded :- UTF8.Encode(decoded);
-    var _ :- RequireEqual([0x61], encoded);
-    var _ :- Require(Uses1Byte(encoded));
+    :- RequireEqual([0x61], encoded);
+    :- Require(Uses1Byte(encoded));
     redecoded :- UTF8.Decode(encoded);
     r := RequireEqual(decoded, redecoded);
   }
 
-  method {:test} Test2Bytes() returns (r: Result<()>) {
+  method {:test} Test2Bytes() returns (r: TestResult) {
     // British pound
     var decoded := "\u00A3";
     var encoded :- UTF8.Encode(decoded);
-    var _ :- RequireEqual([0xC2, 0xA3], encoded);
-    var _ :- Require(Uses2Bytes(encoded));
+    :- RequireEqual([0xC2, 0xA3], encoded);
+    :- Require(Uses2Bytes(encoded));
     var redecoded :- UTF8.Decode(encoded);
-    var _ :- RequireEqual(decoded, redecoded);
+    :- RequireEqual(decoded, redecoded);
 
     // Copyright
     decoded := "\u00A9";
     encoded :- UTF8.Encode(decoded);
-    var _ :- RequireEqual([0xC2, 0xA9], encoded);
-    var _ :- Require(Uses2Bytes(encoded));
+    :- RequireEqual([0xC2, 0xA9], encoded);
+    :- Require(Uses2Bytes(encoded));
     redecoded :- UTF8.Decode(encoded);
-    var _ :- RequireEqual(decoded, redecoded);
+    :- RequireEqual(decoded, redecoded);
 
     // Registered
     decoded := "\u00AE";
     encoded :- UTF8.Encode(decoded);
-    var _ :- RequireEqual([0xC2, 0xAE], encoded);
-    var _ :- Require(Uses2Bytes(encoded));
+    :- RequireEqual([0xC2, 0xAE], encoded);
+    :- Require(Uses2Bytes(encoded));
     redecoded :- UTF8.Decode(encoded);
-    var _ :- RequireEqual(decoded, redecoded);
+    :- RequireEqual(decoded, redecoded);
 
     // Greek Pi
     decoded := "\u03C0";
     encoded :- UTF8.Encode(decoded);
-    var _ :- RequireEqual([0xCF, 0x80], encoded);
-    var _ :- Require(Uses2Bytes(encoded));
+    :- RequireEqual([0xCF, 0x80], encoded);
+    :- Require(Uses2Bytes(encoded));
     redecoded :- UTF8.Decode(encoded);
     r := RequireEqual(decoded, redecoded);
   }
 
-  method {:test} Test3Bytes() returns (r: Result<()>) {
+  method {:test} Test3Bytes() returns (r: TestResult) {
     // Enter symbol
     var decoded := "\u2386";
     var encoded :- UTF8.Encode(decoded);
-    var _ :- RequireEqual([0xE2, 0x8E, 0x86], encoded);
-    var _ :- Require(Uses3Bytes(encoded));
+    :- RequireEqual([0xE2, 0x8E, 0x86], encoded);
+    :- Require(Uses3Bytes(encoded));
     var redecoded :- UTF8.Decode(encoded);
-    var _ :- RequireEqual(decoded, redecoded);
+    :- RequireEqual(decoded, redecoded);
 
     // Alternative key
     decoded := "\u2387";
     encoded :- UTF8.Encode(decoded);
-    var _ :- RequireEqual([0xE2, 0x8E, 0x87], encoded);
-    var _ :- Require(Uses3Bytes(encoded));
+    :- RequireEqual([0xE2, 0x8E, 0x87], encoded);
+    :- Require(Uses3Bytes(encoded));
     redecoded :- UTF8.Decode(encoded);
-    var _ :- RequireEqual(decoded, redecoded);
+    :- RequireEqual(decoded, redecoded);
 
     // Hourglass emoji
     decoded := "\u231B";
     encoded :- UTF8.Encode(decoded);
-    var _ :- RequireEqual([0xE2, 0x8C, 0x9B], encoded);
-    var _ :- Require(Uses3Bytes(encoded));
+    :- RequireEqual([0xE2, 0x8C, 0x9B], encoded);
+    :- Require(Uses3Bytes(encoded));
     redecoded :- UTF8.Decode(encoded);
-    var _ :- RequireEqual(decoded, redecoded);
+    :- RequireEqual(decoded, redecoded);
 
     // Modifier letter cyrillic EN
     decoded := "\u1D78";
     encoded :- UTF8.Encode(decoded);
-    var _ :- RequireEqual([0xE1, 0xB5, 0xB8], encoded);
-    var _ :- Require(Uses3Bytes(encoded));
+    :- RequireEqual([0xE1, 0xB5, 0xB8], encoded);
+    :- Require(Uses3Bytes(encoded));
     redecoded :- UTF8.Decode(encoded);
-    var _ :- RequireEqual(decoded, redecoded);
+    :- RequireEqual(decoded, redecoded);
 
     // Chinese cat (mao)
     decoded := "\u732B";
     encoded :- UTF8.Encode(decoded);
-    var _ :- RequireEqual([0xE7, 0x8C, 0xAB], encoded);
-    var _ :- Require(Uses3Bytes(encoded));
+    :- RequireEqual([0xE7, 0x8C, 0xAB], encoded);
+    :- Require(Uses3Bytes(encoded));
     redecoded :- UTF8.Decode(encoded);
     r := RequireEqual(decoded, redecoded);
   }
 
-  method {:test} Test4Bytes() returns (r: Result<()>) {
+  method {:test} Test4Bytes() returns (r: TestResult) {
     // Cuneiform Sign A - represented as a surrogate of U+12000
     var decoded := "\uD808\uDC00";
     var encoded :- UTF8.Encode(decoded);
-    var _ :- RequireEqual([0xF0, 0x92, 0x80, 0x80], encoded);
-    var _ :- Require(Uses4Bytes(encoded));
+    :- RequireEqual([0xF0, 0x92, 0x80, 0x80], encoded);
+    :- Require(Uses4Bytes(encoded));
     var redecoded :- UTF8.Decode(encoded);
-    var _ :- RequireEqual(decoded, redecoded);
+    :- RequireEqual(decoded, redecoded);
 
     // Mathematical Sans-Serif Bold Italic Small Psi - represented as a surrogate of U+1D7C1
     decoded := "\uD835\uDFC1";
     encoded :- UTF8.Encode(decoded);
-    var _ :- RequireEqual([0xF0, 0x9D, 0x9F, 0x81], encoded);
-    var _ :- Require(Uses4Bytes(encoded));
+    :- RequireEqual([0xF0, 0x9D, 0x9F, 0x81], encoded);
+    :- Require(Uses4Bytes(encoded));
     redecoded :- UTF8.Decode(encoded);
     r := RequireEqual(decoded, redecoded);
   }
